Ongoing: functional lifting definitions

src/variability.lean
@@ -1,17 +1,58 @@
 import data.set
+import data.finset
+
+import .SPL
+
+open SPL
 
 namespace variability
 
-universes u v 
+--constants {Feature : Type} 
+--constants [t : fintype Feature] 
+--constants [d : decidable_eq Feature]
+--constants {L : SPL}
+--parameters (L : SPL Feature)
+ 
+constants {L : SPL}
 
-variables {α β γ : Type}
+section var 
 
-def PC := Prop
+inductive PC : Type
+| All
+| None
+| Atom : Feature → PC 
+| Not  : PC → PC
+| And  : PC → PC → PC
+| Or   : PC → PC → PC 
+ 
+section PCSemantics
 
-structure Var (α : Type u) := 
-    (v : α) (pc : PC) 
+open PC
 
+--def allProducts := allConfigs Feature L
+#check @SPL 
+def semantics : PC → finset Config
+| All           := L.allConfigs
+| None          := ∅
+| (Atom f)      := L.allConfigs.filter (λ p, f ∈ p)
+| (Not pc)      := L.allConfigs.filter (λ p, p ∈ (semantics pc))
+| (And pc₁ pc₂) := (semantics pc₁) ∩ (semantics pc₂)
+| (Or  pc₁ pc₂) := (semantics pc₁) ∪ (semantics pc₂)
+
+end PCSemantics
+
+
+structure Var (α : Type) := (v : α) (pc : PC)
+
+structure Lifted (α : Type) := 
+    (s : list (Var α))
+    (disjoint : ∀ p q : Var α, p ∈ s ∧ q ∈ s ∧ p ≠ q → (semantics (PC.And p.pc q.pc)) = ∅)
+    (complete : semantics(list.foldr (PC.Or) (PC.None) (list.map (Var.pc) s)) = allProducts)
+
+/-
 def set' (α : Type v) : Type v := α → PC
+
+end var
 
 @[class]
 structure has_index (α : Type) {β : Type} :=
@@ -19,7 +60,7 @@ structure has_index (α : Type) {β : Type} :=
 
 def index (s : set' α) (pc : PC) : set α := (and pc) ∘ s
 
-instance : has_index (set' β) := --(set β):= 
+instance : has_index (set' α) := --(set β):= 
 ⟨variability.index⟩ 
 
 protected def mem (x : Var α) (s : set' α) : Prop := 
@@ -48,15 +89,22 @@ def image (f : α → β) (s : set' α) : set' β :=
 
 infix `|`:90 := index
 
-variables (f₁  : set  α → set  β) (f₂  : set  β  → set  γ)
-variables (f₁' : set' α → set' β) (f₂' : set' β  → set' γ)
+variables (f  : set  α → set  β) (g  : set  β  → set  γ)
+variables (f' : set' α → set' β) (g' : set' β  → set' γ)
 theorem fun_comp_correct :
-    (∀ a ρ, (f₁ (a | ρ) = (f₁' a) | ρ)) →
-    (∀ b ρ, (f₂ (b | ρ) = (f₂' b) | ρ)) →
-    (∀ a ρ, (f₂ ∘ f₁) (a | ρ) = ((f₂' ∘ f₁') a) | ρ) :=
+    (∀ a ρ, (f (a | ρ) = (f' a) | ρ)) →
+    (∀ b ρ, (g (b | ρ) = (g' b) | ρ)) →
+    (∀ a ρ, (g ∘ f) (a | ρ) = ((g' ∘ f') a) | ρ) 
+    :=
 begin
 intros h₁ h₂ a ρ, simp, 
 rw h₁, rw← h₂ 
 end
+-/
+
+end var
+
+notation `⟦` p `⟧` := (semantics p)
+postfix `↑`:(max+1) := Lifted
 
 end variability
