src/SPL.lean
@@ -1,0 +1,21 @@
+-- SPL.lean
+-- Software Product Line variability
+import data.fintype
+import data.finset
+
+namespace SPL
+
+variables {Feature : Type}
+variables [d : decidable_eq Feature]
+variables [t : fintype Feature] 
+
+def Config : Type := finset Feature
+
+instance Config_has_mem : has_mem Feature Config := finset.has_mem
+
+structure SPL :=
+    (features : finset Feature)
+    (allFeatures : finset Feature := fintype.elems Feature)
+    (allConfigs : finset Config := allFeatures.powerset)
+
+end SPL
