src/functional.lean
@@ -1,0 +1,64 @@
+-- functional.lean
+-- variability-aware functional programming
+--import .variability
+import data.fintype
+import data.finset
+
+namespace functional
+
+variables {α β : Type}
+
+section func
+
+inductive PC (Feature : Type) : Type
+| All  : PC 
+| None : PC
+| Atom : Feature → PC 
+| Not  : PC → PC
+| And  : PC → PC → PC
+| Or   : PC → PC → PC 
+ 
+def Config (Feature : Type) [fintype Feature] : finset Feature := 
+    fintype.elems Feature
+
+def allConfigs (Feature : Type) [fintype Feature] 
+    := (Config Feature).powerset
+
+--def allProducts := allConfigs Feature L
+
+open PC
+
+def semantics {Feature : Type} [fintype Feature] [decidable_eq Feature]
+    : PC Feature → finset (finset Feature)
+| (All Feature) := allConfigs Feature
+| (None Feature):= ∅
+| (Atom f)      := (allConfigs Feature).filter (λ p, f ∈ p)
+| (Not pc)      := (allConfigs Feature).filter (λ p, p ∈ (semantics pc))
+| (And pc₁ pc₂) := (semantics pc₁) ∩ (semantics pc₂)
+| (Or  pc₁ pc₂) := (semantics pc₁) ∪ (semantics pc₂)
+
+structure Var {Feature: Type} [fintype Feature] (α : Type) := 
+    (v : α) (pc : PC Feature)
+
+structure Lifted {Feature: Type} [fintype Feature] [decidable_eq Feature] (α : Type) := 
+    (s : list (Var α))
+    (disjoint : ∀ p q : Var α, p ∈ s ∧ q ∈ s ∧ p ≠ q → (semantics (And p.pc q.pc)) = ∅)
+    (complete : semantics(list.foldr Or (None Feature) (list.map (Var.pc) s)) = allConfigs Feature)
+
+notation `⟦` p `⟧` := (semantics p)
+postfix `↑`:(max+1) := Lifted
+
+def apply_inner {Feature : Type} [t: fintype Feature] [d: decidable_eq Feature] 
+    (f : @Var Feature t (α → β)) (u : α↑) : list (@Var Feature t β) :=
+    let sat := list.filter (λ(v : Var α), ⟦And f.pc v.pc⟧ ≠ ∅) u.s in
+    list.map (λ(v':Var α), Var.mk (f.v v'.v) (And f.pc  v'.pc)) sat
+
+def apply {Feature : Type} [t: fintype Feature] [d: decidable_eq Feature] 
+    (f : @Lifted Feature t d (α → β)) (v : @Lifted Feature t d α) : @Lifted Feature t d β :=
+    ⟨list.foldr list.append [] (list.map (λ x, apply_inner x v) f.s),
+    _,
+    _⟩
+
+end func
+
+end functional
